src/Std/Data/DTreeMap/Internal/Impl.lean
@@ -43,6 +43,8 @@ inductive WF [Ord α] : Impl α β → Prop where
   | insert {t h k v} : WF t → WF (t.insert k v h).impl
   /-- `erase` preserves well-formedness. Later shown to be subsumed by `.wf`. -/
   | erase {t h k} : WF t → WF (t.erase k h).impl
+  /-- `containsThenInsert` preserves well-formedness. Later shown to be subsumed by `.wf`. -/
+  | containsThenInsert {t h k v} : WF t → WF (t.containsThenInsert k v h).2.impl
 
 /-- A well-formed tree is balanced. This is needed here already because we need to know that the
 tree is balanced to call the optimized modification functions. -/
@@ -51,6 +53,7 @@ theorem WF.balanced [Ord α] {t : Impl α β} : WF t → t.Balanced
   | .empty => balanced_empty
   | .insert _ => TreeB.balanced_impl _
   | .erase _ => TreeB.balanced_impl _
+  | .containsThenInsert _ => TreeB.balanced_impl _
 
 end Impl
 
